---
title: "Untitled"
author: "Andreas C Charitos"
date: "20  2019"
output: pdf_document
---


##Subquestion 3-Posterior up to a constant proportionality and conditional probabilities


##Subquestion 2-Posterior Prior Bayesian Model

we are given that $Y_i \sim N(\mu_i,\sigma^2)~i=1,2,...,n$ $\overrightarrow{~\mu}=(\mu_1,\mu_2,...,\mu_n)$ $p(\mu_1)=1$ $p(\mu_{i+1},\mu_i \sim N(\mu_i,\sigma^2)~~~i=1,2,3,..n-1$

The pdf of the $Y_i$ is given by the formula :
$$f(Y_i/\mu_i,\sigma^2)=\frac{1}{\sqrt 2\pi\sigma^2}e^{-(\frac{(Y_i-\mu_i)^2}{2\sigma^2})}$$

Then the Likekihood is given by :

$$L(Y_1,Y_2,...,Y_n/\mu_i,\sigma^2)=\prod_{i=1}^{n}\frac{1}{\sqrt 2\pi\sigma^2}e^{-(\frac{(Y_i-\mu_i)^2}{\sigma^2})}$$

$$p(\overrightarrow{~Y}/\overrightarrow{~\mu})\propto e^{-(\sum_{i=1}^{n}\frac{(Y_i-\mu_i)^2}{\sigma^2})}(1)$$

We now need to derive the prior which is given by 

$$p(\overrightarrow{~\mu})=p(\mu_1)p(\mu_2/\mu_1)...p(\mu_n/\mu_{n-1})=$$
$$\prod_{i=1}^{n-1}\frac{1}{\sqrt 2\pi\sigma^2}e^{(-\frac{(\mu_{i+1}-\mu_i)^2}{\sigma^2})}$$


$$p(\overrightarrow{~\mu})\propto e^{-(\sum_{i=1}^{n-1}\frac{(\mu_{i+1}-\mu_i)^2}{\sigma^2})}(2)$$


we know that $$Posterior \propto Prior~~Likehihood$$ or

$$p(\overrightarrow{~\mu}/\overrightarrow{~Y})\propto p(\overrightarrow{~Y}/\overrightarrow{~\mu})~~p(\overrightarrow{~\mu})$$ or

$$(1)*(2)=e^{(-\sum_{i=1}^{n-1} \frac{(\mu_{i+1}-\mu_i)^2}{2\sigma^2}-\sum_{i=1}^{n} \frac{(Y_i-\mu_i)^2}{2\sigma^2})}$$


##Subquestion 3-Posterior up to a constant proportionality and conditional probabilities


We know that 
$$p(x_j/x_1,x_2,x_3,...,x_n) \propto\frac{p(x_1,x_2,x_3...,x_n)}{p(x_1,x_2,...,x_{j-1},x_{j+1},...x_n)}$$


using the previous formula we are going to find :

$$p(\mu_n/\overrightarrow{\mu_{-n}}/\overrightarrow{~Y}) \propto \frac{p(\overrightarrow{~\mu}/ \overrightarrow{~Y})}{p(\overrightarrow{~\mu_{-n}}/ \overrightarrow{~Y})}$$


so we have $$\frac{e^{(-\sum_{i=1}^{n-1} \frac{(\mu_{i+1}-\mu_i)^2}{2\sigma^2}-\sum_{i=1}^{n} \frac{(Y_i-\mu_i)^2}{2\sigma^2})}}{e^{(-\sum_{i=1}^{n-2} \frac{(\mu_{i+1}-\mu_i)^2}{2\sigma^2}-\sum_{i=1}^{n-1} \frac{(Y_i-\mu_i)^2}{2\sigma^2})}}=$$

$$e^{-\frac{1}{2\sigma^2} [(\mu_n-\mu_{n-1})^2+(Y_n-\mu_n)^2]}=^{(HINTB)}$$


$$e{-\frac{(\mu_n-(\mu_{n-1}+Y_n)/2)^2}{2\sigma^2/2}} \sim N(\frac{\mu_{n-1+Y_n}}{2},\frac{\sigma^2}{2})$$

Next we need to find 

$$p(\mu_i/\overrightarrow{\mu_{-i}}/\overrightarrow{~Y}) \propto \frac{ p(\overrightarrow{~\mu}/ \overrightarrow{~Y}) }{p(\overrightarrow{~\mu_{-i}}/   \overrightarrow{~Y})}$$

so now we have 

$$\frac{e^{(-\sum_{i=1}^{n-1} \frac{(\mu_{i+1}-\mu_i)^2}{2\sigma^2}-\sum_{i=1}^{n} \frac{(Y_i-\mu_i)^2}{2\sigma^2})}}{e^{(-\sum_{j=i}^{i-2} \frac{(\mu_{j+1}-\mu_j)^2}{2\sigma^2}-\sum_{j=i+1}^{n-1} \frac{(\mu_{j+1}-\mu_j)^2}{2\sigma^2} \sum_{j=1}^{i-1} \frac{(Y_j-\mu_j)^2}{2\sigma^2})- \sum_{j=i+1}^{n} \frac{(Y_j-\mu_j)^2}{2\sigma^2})}}=$$

$$e^{-\frac{1}{2\sigma^2} [(\mu_{i+1}-\mu_{i})^2+(\mu_{i}-\mu_{i-1})^2+(Y_i-\mu_i)^2]}=^{(HINTC)}$$

$$e^{-\frac{(\mu_i-(\mu_{i-1}+Y_i+\mu_{i+1})/3)^2}{2\sigma^2/3}}$$

Using the same steps we obtain also that

$$p(\mu_1/\overrightarrow{\mu_{-1}}/\overrightarrow{~Y}) \propto e^{-\frac{1}{2\sigma^2} [(\mu_2-\mu_1)^2+(Y_1-\mu_1)^2]} \propto e^{-\frac{(\mu_1-(\mu_2+Y_2)/2)^2}{2 \sigma^2/2}}$$





